verified/bitvector_words.s.dfy
@@ -1,0 +1,38 @@
+include "types.s.dfy"
+include "bitvectors.s.dfy"
+
+type shift_amount = s | 0 <= s < 32 // Some shifts allow s=32, but we'll be conservative for simplicity
+
+//-----------------------------------------------------------------------------
+// Functions for bitwise operations
+//-----------------------------------------------------------------------------
+
+function BitwiseXor(x:word, y:word): word
+    { BitsAsWord(BitXor(WordAsBits(x), WordAsBits(y))) }
+
+function BitwiseAnd(x:word, y:word): word
+    { BitsAsWord(BitAnd(WordAsBits(x), WordAsBits(y))) }
+
+function BitwiseOr(x:word, y:word): word
+    { BitsAsWord(BitOr(WordAsBits(x), WordAsBits(y))) }
+
+function BitwiseNot(x:word): word
+    { BitsAsWord(BitNot(WordAsBits(x))) }
+
+function LeftShift(x:word, amount:word): word
+    requires 0 <= amount < 32;
+    { BitsAsWord(BitShiftLeft(WordAsBits(x), amount)) }
+
+function RightShift(x:word, amount:word): word
+    requires 0 <= amount < 32;
+    { BitsAsWord(BitShiftRight(WordAsBits(x), amount)) }
+
+function RotateRight(x:word, amount:shift_amount): word
+    requires 0 <= amount < 32;
+    { BitsAsWord(BitRotateRight(WordAsBits(x), amount)) }
+
+function {:opaque} UpdateTopBits(origval:word, newval:word): word
+{
+    BitwiseOr(LeftShift(newval, 16), BitwiseMaskLow(origval, 16))
+}
+
