verified/bitvectors.i.dfy
@@ -1,15 +1,22 @@
 include "bitvectors.s.dfy"
-include "ARMdef.s.dfy"
+include "bitvector_words.s.dfy"
+include "bitvectors_primitive.i.dfy"
 
 lemma lemma_BitShiftsRightSum(x: bv32, a: nat, b: nat)
     requires 0 <= a + b < 32
     ensures BitShiftRight(x, a + b) == BitShiftRight(BitShiftRight(x, a), b)
-{ reveal BitShiftRight(); }
+{
+    lemma_ShiftsRightSum(x, a, b);
+    reveal BitShiftRight();
+}
 
 lemma lemma_BitShiftsLeftSum(x: bv32, a: nat, b: nat)
     requires 0 <= a + b < 32
     ensures BitShiftLeft(x, a + b) == BitShiftLeft(BitShiftLeft(x, a), b)
-{ reveal BitShiftLeft(); }
+{
+    lemma_ShiftsLeftSum(x, a, b);
+    reveal BitShiftLeft();
+}
 
 lemma lemma_BitOrCommutative(a: bv32, b:bv32)
     ensures BitOr(a, b) == BitOr(b, a)
@@ -323,8 +330,9 @@ lemma lemma_BitwiseOrAssociative(a: word, b: word, c: word)
 }
 
 lemma lemma_BitsAndWordConversions()
+    // to avoid matching loops, we give of these a more restrictive trigger:
     ensures forall w:word :: BitsAsWord(WordAsBits(w)) == w;
-    ensures forall b:bv32 :: WordAsBits(BitsAsWord(b)) == b;
+    ensures forall b:bv32 {:trigger WordAsBits(BitsAsWord(b))} :: WordAsBits(BitsAsWord(b)) == b;
 {
     forall w:word 
         ensures BitsAsWord(WordAsBits(w)) == w;
@@ -338,60 +346,31 @@ lemma lemma_BitsAndWordConversions()
     }
 }
 
-lemma lemma_shift16maskhigh(x:bv32)
-    requires 0 <= x <= 0xffffffff
-    ensures (x >> 16) << 16 == x & 0xffff0000
-{}
-
-lemma lemma_masklow16(c:word)
-    ensures BitwiseMaskLow(c % 0x10000, 16) == BitsAsWord(WordAsBits(c) & 0xffff)
+lemma lemma_load_32_bit_const_bv(c:bv32)
+    ensures c == BitOr(BitShiftLeft(BitShiftRight(c, 16), 16), BitAnd(BitMod(c, 0x10000), 0xffff))
 {
-    ghost var cb := WordAsBits(c);
-    assert WordAsBits(0x10000) == 0x10000 by { reveal WordAsBits(); }
-    calc {
-        BitwiseMaskLow(c % 0x10000, 16);
-        { reveal BitwiseMaskLow(); }
-        BitsAsWord(BitAnd(WordAsBits(c % 0x10000), BitmaskLow(16)));
-        { assert BitmaskLow(16) == 0xffff by { reveal BitAtPos(); } }
-        BitsAsWord(BitAnd(WordAsBits(c % 0x10000), 0xffff));
-        { lemma_BitModEquiv(c, 0x10000); }
-        BitsAsWord(BitAnd(WordAsBits(BitsAsWord(BitMod(cb, 0x10000))), 0xffff));
-        { lemma_BitsAsWordAsBits(BitMod(cb, 0x10000)); }
-        BitsAsWord(BitAnd(BitMod(cb, 0x10000), 0xffff));
-        { reveal BitAnd(); reveal BitMod(); }
-        BitsAsWord(cb & 0xffff);
-    }
+    reveal BitOr();
+    reveal BitAnd();
+    reveal BitShiftLeft();
+    reveal BitShiftRight();
+    reveal BitMod();
+}
+
+lemma lemma_load_32_bit_const_word(c:word)
+    ensures c == UpdateTopBits(c % 0x10000, BitsAsWord(BitShiftRight(WordAsBits(c), 16)))
+{
+    assert BitmaskLow(16) == 0xffff by { reveal BitAtPos(); }
+    assert BitsAsWord(0x10000) == 0x10000 by { reveal BitsAsWord(); }
+    reveal UpdateTopBits();
+    reveal BitwiseMaskLow();
+    lemma_BitModEquiv(c, 0x10000);
+    lemma_load_32_bit_const_bv(WordAsBits(c));
+    lemma_BitsAndWordConversions();
 }
 
 lemma lemma_load_32_bit_const(c:word)
     ensures c == UpdateTopBits(c % 0x10000, BitsAsWord(WordAsBits(c) >> 16))
 {
-    ghost var bottom := c % 0x10000;
-    ghost var cb := WordAsBits(c);
-    ghost var top := BitsAsWord(cb >> 16);
-
-    assert BitsAsWord(0x10000) == 0x10000 by { reveal BitsAsWord(); }
-    lemma_WordBitEquiv(0x10000, 0x10000);
-
-    calc {
-        UpdateTopBits(bottom, top);
-        { reveal UpdateTopBits(); }
-        BitwiseOr(LeftShift(top, 16), BitwiseMaskLow(bottom, 16));
-        { calc {
-                LeftShift(top, 16);
-                { reveal BitShiftLeft(); }
-                BitsAsWord(WordAsBits(BitsAsWord(cb >> 16)) << 16);
-                { lemma_BitsAsWordAsBits(cb >> 16); lemma_shift16maskhigh(cb); }
-                BitsAsWord(cb & 0xffff0000);
-        } }
-        BitwiseOr(BitsAsWord(cb & 0xffff0000), BitwiseMaskLow(bottom, 16));
-        { lemma_masklow16(c); }
-        BitwiseOr(BitsAsWord(cb & 0xffff0000), BitsAsWord(cb & 0xffff));
-        { lemma_BitsAndWordConversions(); }
-        BitsAsWord(BitOr(cb & 0xffff0000, cb & 0xffff));
-        { reveal BitOr(); }
-        BitsAsWord(cb);
-        { lemma_WordAsBitsAsWord(c); }
-        c;
-    }
+    lemma_load_32_bit_const_word(c);
+    reveal BitShiftRight();
 }
